tester halfly done

verification/Tester.dfy
@@ -1,12 +1,43 @@
 include "UntestedBloodList.dfy"
 include "TestingBloodList.dfy"
 include "TestedBloodList.dfy"
+include "UntestedBlood.dfy"
+include "TestingBlood.dfy"
+include "TestedBlood.dfy"
 
 // remove from untested, add to testing
 // Correspond to Tester.py::startTest()
-method startTest(id: int, untestedlist: UntestedBloodList, testing: TestingBloodList)
+// Use startTime to represent current time
+method startTest(id: int, startTime: int, untestedlist: UntestedBloodList, testing: TestingBloodList)
+    requires untestedlist != null;
+    requires testing != null;
+    requires untestedlist.Valid();
+    requires testing.Valid();
+    requires untestedlist.UniqueId();
+    requires testing.UniqueId();
+    requires exists t :: (0 <= t < untestedlist.upto && untestedlist.list[t].id == id);
+    requires forall t :: (0 <= t < untestedlist.upto && untestedlist.list[t].id == id ) ==> (untestedlist.list[t].retrieval < startTime);
+    requires forall i :: 0 <= i < untestedlist.upto  ==> 
+        (forall k :: 0 <= k < testing.upto ==> 
+        untestedlist.list[i].id != testing.list[k].id);
+    modifies untestedlist;
+    modifies untestedlist.list;
+    modifies untestedlist`upto;
+    modifies testing;
+    modifies testing.list;
+    modifies testing`upto;
+    ensures untestedlist.Valid();
+    ensures testing.Valid();
+    ensures untestedlist.UniqueId();
+    ensures testing.UniqueId();
+    ensures untestedlist != null;
+    ensures testing != null;
+    ensures untestedlist.list == old(untestedlist.list); 
+    ensures testing.list == old(testing.list) || fresh(testing.list);
 {
-
+    var extracted := untestedlist.extractBlood(id);
+    var newBlood := new TestingBlood(id, extracted.retrieval, startTime);
+    testing.addBlood(newBlood);
 }
 
 // remove from testing, add to tested
